src/Database/Proof/DataStructureSpecs.v
@@ -15,16 +15,44 @@ Section lifting.
   Admitted.
 
   Theorem wp_readIORef T (r: IORef T) (x ret:T) :
-    {{{ r ↦ x }}}
+    {{{ ▷ r ↦ x }}}
       Data.readIORef r
       {{{ RET ret; ⌜ret = x⌝ ∗ r ↦ x }}}.
   Proof.
   Admitted.
 
   Theorem wp_writeIORef T (r: IORef T) (x x':T) :
-    {{{ r ↦ x }}}
+    {{{ ▷ r ↦ x }}}
       Data.writeIORef r x'
       {{{ RET (); r ↦ x' }}}.
+  Proof.
+  Admitted.
+
+  Theorem wp_newArray T (r:Array T) :
+    {{{ emp }}}
+      Data.newArray T
+      {{{ RET r; r ↦ [] }}}.
+  Proof.
+  Admitted.
+
+  Theorem wp_arrayLength T (r:Array T) (v: list T) (l:uint64) :
+    {{{ ▷ r ↦ v }}}
+      Data.arrayLength r
+      {{{ RET l; ⌜l = fromNum (length v)⌝ ∗ r ↦ v }}}.
+  Proof.
+  Admitted.
+
+  Theorem wp_arrayGet T (r:Array T) (v: list T) (i:uint64) (x:T) :
+    {{{ ▷ r ↦ v ∗ ⌜toNum i < length v⌝ }}}
+      Data.arrayGet r i
+      {{{ RET x; ⌜List.nth_error v i.(toNum) = Some x⌝ ∗ r ↦ v }}}.
+  Proof.
+  Admitted.
+
+  Theorem wp_arrayAppend T (r:Array T) (v: list T) (x:T) :
+    {{{ ▷ r ↦ v }}}
+      Data.arrayAppend r x
+      {{{ RET (); r ↦ (v ++ [x]) }}}.
   Proof.
   Admitted.
 
